Adjust flat_to_clos to produce Constant ops

compiler/backend/flat_to_closScript.sml
@@ -35,12 +35,14 @@ Proof
 QED
 
 Definition compile_lit_def:
-  compile_lit t (IntLit i) = closLang$Op t (Const i) [] /\
-  compile_lit t (Char c) = closLang$Op t (Const (& (ORD c))) [] /\
-  compile_lit t (StrLit s) = closLang$Op t (String s) [] /\
-  compile_lit t (Word8 b) = closLang$Op t (Const (& (w2n b))) [] /\
-  compile_lit t (Word64 w) =
-    closLang$Op t WordFromInt [closLang$Op t (Const (& (w2n w))) []]
+  compile_lit t l =
+    closLang$Op t (Constant $
+    dtcase l of
+    | IntLit i => ConstInt i
+    | Char c => ConstInt (& (ORD c))
+    | StrLit s => ConstStr s
+    | Word8 b => ConstInt (& (w2n b))
+    | Word64 w => ConstWord64 w) []
 End
 
 Definition arg1_def:
@@ -218,6 +220,35 @@ Proof
   Cases_on ‘op’ \\ fs [dest_nop_def] \\ every_case_tac \\ fs []
 QED
 
+Definition dest_Constant_def:
+  dest_Constant (Op t (Constant c) []) = SOME c ∧
+  dest_Constant _ = NONE
+End
+
+Theorem dest_Constant_pmatch:
+  dest_Constant xs = case xs of Op t (Constant x) [] => SOME x | _ => NONE
+Proof
+  CONV_TAC(RAND_CONV patternMatchesLib.PMATCH_ELIM_CONV)
+  \\ every_case_tac \\ fs [dest_Constant_def]
+QED
+
+Definition dest_Constants_def:
+  dest_Constants [] = SOME [] ∧
+  dest_Constants (c::cs) =
+    dtcase dest_Constant c of
+    | NONE => NONE
+    | SOME x => dtcase dest_Constants cs of
+                | NONE => NONE
+                | SOME xs => SOME (x::xs)
+End
+
+Definition SmartCons_def:
+  SmartCons t tag xs =
+    dtcase dest_Constants xs of
+    | NONE => Op t (Cons tag) xs
+    | SOME cs => Op t (Constant (ConstCons tag (REVERSE cs))) []
+End
+
 Definition compile_def:
   (compile m [] = []) /\
   (compile m (x::y::xs) = compile m [x] ++ compile m (y::xs)) /\
@@ -226,7 +257,7 @@ Definition compile_def:
   (compile m [Var_local t v] = [Var t (findi (SOME v) m)]) /\
   (compile m [Con t n es] =
      let tag = (dtcase n of SOME (t,_) => t | _ => 0) in
-       [Op t (Cons tag) (compile m (REVERSE es))]) /\
+       [SmartCons t tag (compile m (REVERSE es))]) /\
   (compile m [App t op es] =
      dtcase dest_nop op es of
      | SOME e => compile m [e]
